src/Bedrock/End2End/X25519/GarageDoor.v
@@ -19,14 +19,11 @@ Require Import Crypto.Bedrock.End2End.X25519.Field25519.
 Require Import Crypto.Bedrock.End2End.X25519.MontgomeryLadder.
 Require Import bedrock2Examples.LAN9250.
 Require Import bedrock2Examples.lightbulb.
-(*TODO: remove*)
 Require Import bedrock2Examples.chacha20.
 Require Import bedrock2Examples.memequal.
 Require Import bedrock2Examples.memswap.
 Require Import bedrock2Examples.memconst.
 Require Import Rupicola.Examples.Net.IPChecksum.IPChecksum.
-
-
 
 Local Open Scope string_scope.
 Import Syntax Syntax.Coercions NotationsCustomEntry.
@@ -91,7 +88,7 @@ Definition loopfn := func! {
     output! MMIOWRITE($0x1001200c, mmio_val | (set1<<$1 | set0) << $11);
 
     if (set0|set1) { (* rekey *)
-        chacha20_block(st, st, (*nonce*)pk) (* NOTE: another impl? *)
+        chacha20_block(st, st, (*nonce*)pk, $0) (* NOTE: another impl? *)
     }
   }
 }.
@@ -219,16 +216,14 @@ Local Instance spec_of_lan9250_tx : spec_of "lan9250_tx" := spec_of_lan9250_tx.
 Local Instance spec_of_memswap : spec_of "memswap" := spec_of_memswap.
 Local Instance spec_of_memequal : spec_of "memequal" := spec_of_memequal.
 
-(*
 Local Instance spec_of_chacha20 : spec_of "chacha20_block" :=
-  fnspec! "chacha20_block" out key nonce / (pt k n : list Byte.byte) (R Rk Rn : map.rep -> Prop),
+  fnspec! "chacha20_block" out key nonce counter / (pt k n : list Byte.byte) (R Rk Rn : map.rep -> Prop),
   { requires t m :=
       m =* pt$@out * R /\ length pt = 64%nat /\
       m =* k$@key * Rk /\ length k = 32%nat /\
-          (*TODO: account for difference in nonce length*)
       m =* n$@nonce * Rn /\ length n = 12%nat;
     ensures T m := T = t /\ exists ct, m =* ct$@out * R /\ length ct = 64%nat /\
-      ct = RupicolaCrypto.Spec.chacha20_block k n }.*)
+      ct = RupicolaCrypto.Spec.chacha20_encrypt k (Z.to_nat (word.unsigned counter)) n pt }.
 
 Definition memrep bs R : state -> map.rep(map:=SortedListWord.map _ _) -> Prop := fun '(seed, sk) m =>
   m =*
@@ -252,12 +247,6 @@ Import ZnWords.
 Import coqutil.Tactics.autoforward.
 
 Import Crypto.Util.FixCoqMistakes.
-
-
-Require Crypto.Bedrock.End2End.RupicolaCrypto.ChaChaWrapped.
-Import ChaChaWrapped (spec_of_chacha20).
-
-Local Existing Instance spec_of_chacha20.
 
 Lemma loopfn_ok : program_logic_goal_for_function! loopfn.
 Proof.
@@ -930,22 +919,18 @@ Definition loop := func! { loopfn() } .
 Definition memconst_pk := memconst garageowner.
 Definition ip_checksum := ip_checksum_br2fn.
 
-
 Definition funcs :=
   &[, init; loop;
     initfn; loopfn;
     memswap; memequal; memconst_pk;
     ip_checksum;
-    chacha20_block_wrapped; quarter_body;
+    chacha20_block; chacha20_quarter;
     lan9250_tx ]
     ++lightbulb.function_impls
     ++MontgomeryLadder.funcs.
 
-(*
-Lemma chacha20_ok: forall functions, spec_of_chacha20 (&,chacha20_block_body::&,quarter_body::functions).
-Proof.
+Lemma chacha20_ok: forall functions, spec_of_chacha20 (&,chacha20_block::&,chacha20_quarter::functions).
 Admitted.
-*)
 
 Import SPI.
 Lemma link_loopfn : spec_of_loopfn funcs.
